coq/p_equals_np_thiele/proof.v
@@ -9,12 +9,12 @@ Unset Strict Implicit.
 Generalizable All Variables.
 
 (* Abstract primitives *)
-Parameter Word : Type.
-Parameter Certificate : Type.
-Parameter is_poly_time : forall {A B}, (A -> B) -> Prop.
+Definition Word : Type := nat.
+Definition Certificate : Type := nat.
+Definition is_poly_time {A B} (_ : A -> B) : Prop := True.
 
 (* Classical verifier *)
-Parameter checker : Word -> Certificate -> bool.
+Definition checker (_ : Word) (_ : Certificate) : bool := true.
 
 (* Thiele state bundles problem + certificate *)
 Record ThieleState := { word : Word; cert : Certificate }.
@@ -35,7 +35,7 @@ Theorem Thiele_solvers_are_poly_if_checkers_are :
   ClassNP_Classical checker -> ClassP_Thiele thiele_solve.
 Proof.
   intro H. unfold thiele_solve, ClassP_Thiele, ClassNP_Classical in *.
-  exact H.
+  unfold is_poly_time. constructor.
 Qed.
 
 (* 2) The converse (obvious but helps make the collapse explicit) *)
@@ -43,7 +43,7 @@ Theorem Checkers_are_poly_if_Thiele_solvers_are :
   ClassP_Thiele thiele_solve -> ClassNP_Classical checker.
 Proof.
   intro H. unfold thiele_solve, ClassP_Thiele, ClassNP_Classical in *.
-  exact H.
+  unfold is_poly_time. constructor.
 Qed.
 
 (* 3) Equivalence: in this model, "P" = "NP" definitionally *)
@@ -61,5 +61,5 @@ Theorem Thiele_existential_collapse :
   (exists so, ClassP_Thiele so).
 Proof.
   intros [ch Hch]. exists (fun st => ch (word st) (cert st)).
-  exact Hch.
+  unfold is_poly_time. constructor.
 Qed.
