coq/sight_hierarchy/FractalSight.v
@@ -1,0 +1,6 @@
+(* FractalSight.v - Placeholder for fractal sight hierarchy proofs *)
+
+Require Import Coq.Init.Logic.
+
+Lemma fractal_sight_placeholder : True.
+Proof. exact I. Qed.
