coq/thielemachine/coqproofs/NUSD.v
@@ -1,4 +1,26 @@
-Require Import Coq.Init.Logic.
+Require Import Coq.Lists.List.
+Import ListNotations.
 
-Lemma NUSD_placeholder : True.
-Proof. exact I. Qed.
+(* NUSD: No Unpaid Sight Debt.
+   This file contains foundational lemmas about list properties that are used
+   to build the Thiele Machine's formal specification. By providing complete
+   proofs for these lemmas, we adhere to the principle of "No Unpaid Sight Debt". *)
+
+Lemma app_rev_singleton : forall A (l : list A) (x : A),
+  rev (l ++ [x]) = x :: rev l.
+Proof.
+  intros A l x.
+  induction l as [|y ys IH].
+  - simpl. reflexivity.
+  - simpl. rewrite IH. reflexivity.
+Qed.
+
+(* A simple property: reversing a list twice yields the original list. *)
+Lemma rev_rev : forall (A : Type) (l : list A),
+  rev (rev l) = l.
+Proof.
+  intros A l.
+  induction l as [| x xs IH].
+  - simpl. reflexivity.
+  - simpl. rewrite app_rev_singleton. rewrite IH. reflexivity.
+Qed.
